concordium/src/concordium_prims.rs
@@ -1,69 +1,23 @@
-#[cfg(not(feature = "hacspec"))]
+#![feature(register_tool)]
+#![register_tool(hax)]
+
+#[hax_lib_macros::skip]
+extern crate hax_lib_macros;
+#[hax_lib_macros::skip]
+use hax_lib_macros::*;
+
+#[skip]
 use crate::*;
 
-use hacspec_lib::*;
-
-#[cfg(not(feature = "hacspec"))]
-pub fn coerce_rust_to_hacspec_public_byte_seq(buf: &[u8]) -> PublicByteSeq {
-    PublicByteSeq::from_native_slice(buf)
-}
-
-// TODO: Make creusot friendly version
-#[cfg(not(feature = "hacspec"))]
-pub fn coerce_hacspec_to_rust_public_byte_seq(buf: PublicByteSeq) -> Vec<u8> {
-    // buf.native_slice().iter().collect();
-    let mut temp_vec: Vec<u8> = Vec::new();
-    for i in 0..buf.len() {
-        temp_vec.push(buf.index(i).clone())
-    }
-    temp_vec
-}
-
-#[cfg(not(feature = "hacspec"))]
 extern "C" {
     pub(crate) fn accept() -> u32;
 }
 
-#[cfg(not(feature = "hacspec"))]
-#[trusted]
-pub(crate) fn accept_creusot() -> u32 {
-    unsafe { accept() }
-}
-
-#[cfg(feature = "hacspec")]
-pub(crate) fn accept_hacspec() -> u32 {
-    1u32
-}
-
-#[cfg(not(feature = "hacspec"))]
-pub(crate) fn accept_hacspec() -> u32 {
-    accept_creusot()
-}
-
-#[cfg(not(feature = "hacspec"))]
 extern "C" {
   // Basic action to send tokens to an account.
   pub(crate) fn simple_transfer(addr_bytes: *const u8, amount: u64) -> u32;
 }
 
-#[cfg(not(feature = "hacspec"))]
-#[trusted]
-pub(crate) fn simple_transfer_creusot(addr_bytes: *const u8, amount: u64) -> u32 {
-    unsafe { simple_transfer(addr_bytes, amount) }
-}
-
-#[cfg(feature = "hacspec")]
-pub(crate) fn simple_transfer_hacspec(buf: PublicByteSeq, amount: u64) -> u32 {
-    1u32
-}
-
-#[cfg(not(feature = "hacspec"))]
-pub(crate) fn simple_transfer_hacspec(buf: PublicByteSeq, amount: u64) -> u32 {
-    let temp = &mut coerce_hacspec_to_rust_public_byte_seq(buf.clone())[..];
-    simple_transfer_creusot(temp.as_ptr(), amount)
-}
-
-#[cfg(not(feature = "hacspec"))]
 extern "C" {
   // Send a message to a smart contract.
   pub(crate) fn send(
@@ -77,113 +31,23 @@ extern "C" {
   ) -> u32;
 }
 
-#[cfg(not(feature = "hacspec"))]
-#[trusted]
-pub(crate) fn send_creusot(
-      addr_index: u64,
-      addr_subindex: u64,
-      receive_name: *const u8,
-      receive_name_len: u32,
-      amount: u64,
-      parameter: *const u8,
-      parameter_len: u32,
-  ) -> u32 {
-    unsafe { send(addr_index, addr_subindex, receive_name, receive_name_len, amount, parameter, parameter_len) }
-}
-
-#[cfg(feature = "hacspec")]
-pub(crate) fn send_hacspec(
-      addr_index: u64,
-      addr_subindex: u64,
-      receive_name: PublicByteSeq,
-      amount: u64,
-      parameter: PublicByteSeq,
-  ) -> u32 {
-    1u32
-}
-
-#[cfg(not(feature = "hacspec"))]
-pub(crate) fn send_hacspec(
-      addr_index: u64,
-      addr_subindex: u64,
-      receive_name: PublicByteSeq,
-      amount: u64,
-      parameter: PublicByteSeq,
-  ) -> u32 {
-    let temp_receive_name = &mut coerce_hacspec_to_rust_public_byte_seq(receive_name.clone())[..];
-    let temp_parameter = &mut coerce_hacspec_to_rust_public_byte_seq(parameter.clone())[..];
-    send_creusot(addr_index, addr_subindex, temp_receive_name.as_ptr(), receive_name.len() as u32, amount, temp_parameter.as_ptr(), parameter.len() as u32)
-}
-
-#[cfg(not(feature = "hacspec"))]
 extern "C" {
   // Combine two actions using normal sequencing. This is using the stack of
   // actions already produced.
   pub(crate) fn combine_and(l: u32, r: u32) -> u32;
 }
 
-#[cfg(not(feature = "hacspec"))]
-#[trusted]
-pub(crate) fn combine_and_creusot(l: u32, r: u32) -> u32 {
-    unsafe { combine_and(l, r) }
-}
-
-#[cfg(feature = "hacspec")]
-pub(crate) fn combine_and_hacspec(l: u32, r: u32) -> u32 {
-    1u32
-}
-
-#[cfg(not(feature = "hacspec"))]
-pub(crate) fn combine_and_hacspec(l: u32, r: u32) -> u32 {
-    combine_and_creusot(l,r)
-}
-
-#[cfg(not(feature = "hacspec"))]
 extern "C" {
   // Combine two actions using normal sequencing. This is using the stack of
   // actions already produced.
   pub(crate) fn combine_or(l: u32, r: u32) -> u32;
 }
 
-#[cfg(not(feature = "hacspec"))]
-#[trusted]
-pub(crate) fn combine_or_creusot(l: u32, r: u32) -> u32 {
-    unsafe { combine_or(l, r) }
-}
-
-#[cfg(feature = "hacspec")]
-pub(crate) fn combine_or_hacspec(l: u32, r: u32) -> u32 {
-    1u32
-}
-
-#[cfg(not(feature = "hacspec"))]
-pub(crate) fn combine_or_hacspec(l: u32, r: u32) -> u32 {
-    combine_or_creusot(l,r)
-}
-
-#[cfg(not(feature = "hacspec"))]
 extern "C" {
     // Get the size of the parameter to the method (either init or receive).
     pub(crate) fn get_parameter_size() -> u32;
 }
 
-#[cfg(not(feature = "hacspec"))]
-#[trusted]
-pub(crate) fn get_parameter_size_creusot() -> u32 {
-    unsafe { get_parameter_size() }
-}
-
-#[cfg(feature = "hacspec")]
-pub(crate) fn get_parameter_size_hacspec() -> u32 {
-    1u32
-}
-
-#[cfg(not(feature = "hacspec"))]
-pub(crate) fn get_parameter_size_hacspec() -> u32 {
-    get_parameter_size_creusot()
-}
-
-#[cfg(not(feature = "hacspec"))]
 extern "C" {
     // Write a section of the parameter to the given location. Return the number
     // of bytes written. The location is assumed to contain enough memory to
@@ -191,28 +55,6 @@ extern "C" {
     pub(crate) fn get_parameter_section(param_bytes: *mut u8, length: u32, offset: u32) -> u32;
 }
 
-#[cfg(not(feature = "hacspec"))]
-#[trusted]
-pub(crate) fn get_parameter_section_creusot(start: *mut u8, length: u32, offset: u32) -> u32 {
-    unsafe { get_parameter_section(start, length, offset) }
-}
-
-#[cfg(feature = "hacspec")]
-pub(crate) fn get_parameter_section_hacspec(buf: PublicByteSeq, offset: u32) -> (PublicByteSeq, u32) {
-    (buf, 1u32)
-}
-
-#[cfg(not(feature = "hacspec"))]
-pub(crate) fn get_parameter_section_hacspec(buf: PublicByteSeq, offset: u32) -> (PublicByteSeq, u32) {
-    let temp = &mut coerce_hacspec_to_rust_public_byte_seq(buf.clone())[..];
-    let result = get_parameter_section_creusot(temp.as_mut_ptr(), buf.len() as u32, offset);
-    (
-        coerce_rust_to_hacspec_public_byte_seq(&temp),
-        result,
-    )
-}
-
-#[cfg(not(feature = "hacspec"))]
 extern "C" {
   // Write a section of the policy to the given location. Return the number
   // of bytes written. The location is assumed to contain enough memory to
@@ -220,28 +62,6 @@ extern "C" {
   pub(crate) fn get_policy_section(policy_bytes: *mut u8, length: u32, offset: u32) -> u32;
 }
 
-#[cfg(not(feature = "hacspec"))]
-#[trusted]
-pub(crate) fn get_policy_section_creusot(policy_bytes: *mut u8, length: u32, offset: u32) -> u32 {
-    unsafe { get_policy_section(policy_bytes, length, offset) }
-}
-
-#[cfg(feature = "hacspec")]
-pub(crate) fn get_policy_section_hacspec(policy_bytes: PublicByteSeq, offset: u32) -> (PublicByteSeq, u32) {
-    (policy_bytes, 1u32)
-}
-
-#[cfg(not(feature = "hacspec"))]
-pub(crate) fn get_policy_section_hacspec(policy_bytes: PublicByteSeq, offset: u32) -> (PublicByteSeq, u32) {
-    let temp = &mut coerce_hacspec_to_rust_public_byte_seq(policy_bytes.clone())[..];
-    let result = get_policy_section_creusot(temp.as_mut_ptr(), policy_bytes.len() as u32, offset);
-    (
-        coerce_rust_to_hacspec_public_byte_seq(&temp),
-        result,
-    )
-}
-
-#[cfg(not(feature = "hacspec"))]
 extern "C" {
     // Add a log item. Return values are
     // - -1 if logging failed due to the message being too long
@@ -250,71 +70,14 @@ extern "C" {
     pub(crate) fn log_event(start: *const u8, length: u32) -> i32;
 }
 
-#[cfg(not(feature = "hacspec"))]
-#[trusted]
-pub(crate) fn log_event_creusot(start: *const u8, length: u32) -> i32 {
-    unsafe { log_event(start, length) }
-}
-
-#[cfg(feature = "hacspec")]
-pub(crate) fn log_event_hacspec(start: PublicByteSeq) -> (PublicByteSeq, i32) {
-    (start, 1i32)
-}
-
-#[cfg(not(feature = "hacspec"))]
-pub(crate) fn log_event_hacspec(start: PublicByteSeq) -> (PublicByteSeq, i32) {
-    let temp = &mut coerce_hacspec_to_rust_public_byte_seq(start.clone())[..];
-    let result = log_event_creusot(temp.as_ptr(), start.len() as u32);
-    (coerce_rust_to_hacspec_public_byte_seq(&temp), result)
-}
-
-#[cfg(not(feature = "hacspec"))]
 extern "C" {
     pub(crate) fn load_state(start: *mut u8, length: u32, offset: u32) -> u32;
 }
 
-#[cfg(not(feature = "hacspec"))]
-#[trusted]
-pub(crate) fn load_state_creusot(start: *mut u8, length: u32, offset: u32) -> u32 {
-    unsafe { load_state(start, length, offset) }
-}
-
-#[cfg(feature = "hacspec")]
-pub(crate) fn load_state_hacspec(buf: PublicByteSeq, offset: u32) -> (PublicByteSeq, u32) {
-    (buf, 1u32)
-}
-
-#[cfg(not(feature = "hacspec"))]
-pub(crate) fn load_state_hacspec(buf: PublicByteSeq, offset: u32) -> (PublicByteSeq, u32) {
-    let temp = &mut coerce_hacspec_to_rust_public_byte_seq(buf.clone())[..];
-    let result = load_state_creusot(temp.as_mut_ptr(), buf.len() as u32, offset);
-    (coerce_rust_to_hacspec_public_byte_seq(&temp), result)
-}
-
-#[cfg(not(feature = "hacspec"))]
 extern "C" {
     pub(crate) fn write_state(start: *mut u8, length: u32, offset: u32) -> u32;
 }
 
-#[cfg(not(feature = "hacspec"))]
-#[trusted]
-pub(crate) fn write_state_creusot(start: *mut u8, length: u32, offset: u32) -> u32 {
-    unsafe { write_state(start, length, offset) }
-}
-
-#[cfg(feature = "hacspec")]
-pub(crate) fn write_state_hacspec(buf: PublicByteSeq, offset: u32) -> (PublicByteSeq, u32) {
-    (buf, 1u32)
-}
-
-#[cfg(not(feature = "hacspec"))]
-pub(crate) fn write_state_hacspec(buf: PublicByteSeq, offset: u32) -> (PublicByteSeq, u32) {
-    let temp = &mut coerce_hacspec_to_rust_public_byte_seq(buf.clone())[..];
-    let result = write_state_creusot(temp.as_mut_ptr(), buf.len() as u32, offset);
-    (coerce_rust_to_hacspec_public_byte_seq(&temp), result)
-}
-
-#[cfg(not(feature = "hacspec"))]
 extern "C" {
     // Resize state to the new value (truncate if new size is smaller). Return 0 if
     // this was unsuccesful (new state too big), or 1 if successful.
@@ -322,181 +85,38 @@ extern "C" {
                                                       // get current state size in bytes.
 }
 
-#[cfg(not(feature = "hacspec"))]
-#[trusted]
-pub(crate) fn resize_state_creusot(new_size: u32) -> u32 {
-    unsafe { resize_state(new_size) }
-}
-
-#[cfg(feature = "hacspec")]
-pub(crate) fn resize_state_hacspec(new_size: u32) -> u32 {
-    1u32
-}
-
-#[cfg(not(feature = "hacspec"))]
-pub(crate) fn resize_state_hacspec(new_size: u32) -> u32 {
-    resize_state_creusot(new_size)
-}
-
-#[cfg(not(feature = "hacspec"))]
 extern "C" {
     pub(crate) fn state_size() -> u32;
 }
 
-#[cfg(not(feature = "hacspec"))]
-#[trusted]
-pub(crate) fn state_size_creusot() -> u32 {
-    unsafe { state_size() }
-}
-
-#[cfg(feature = "hacspec")]
-pub(crate) fn state_size_hacspec() -> u32 {
-    1u32
-}
-
-#[cfg(not(feature = "hacspec"))]
-pub(crate) fn state_size_hacspec() -> u32 {
-    state_size_creusot()
-}
-
-#[cfg(not(feature = "hacspec"))]
 extern "C" {
   // Getter for the init context.
   /// Address of the sender, 32 bytes
   pub(crate) fn get_init_origin(start: *mut u8);
 }
 
-#[cfg(not(feature = "hacspec"))]
-#[trusted]
-pub(crate) fn get_init_origin_creusot(start: *mut u8) {
-    unsafe { get_init_origin(start) }
-}
-
-#[cfg(feature = "hacspec")]
-pub(crate) fn get_init_origin_hacspec(start: PublicByteSeq) -> PublicByteSeq {
-    start
-}
-
-#[cfg(not(feature = "hacspec"))]
-pub(crate) fn get_init_origin_hacspec(start: PublicByteSeq) -> PublicByteSeq {
-    let temp = &mut coerce_hacspec_to_rust_public_byte_seq(start.clone())[..];
-    get_init_origin_creusot(temp.as_mut_ptr());
-    coerce_rust_to_hacspec_public_byte_seq(&temp)
-}
-
-#[cfg(not(feature = "hacspec"))]
 extern "C" {
   /// Invoker of the top-level transaction, AccountAddress.
   pub(crate) fn get_receive_invoker(start: *mut u8);
 }
 
-#[cfg(not(feature = "hacspec"))]
-#[trusted]
-pub(crate) fn get_receive_invoker_creusot(start: *mut u8) {
-    unsafe { get_receive_invoker(start) }
-}
-
-#[cfg(feature = "hacspec")]
-pub(crate) fn get_receive_invoker_hacspec(start: PublicByteSeq) -> PublicByteSeq {
-    start
-}
-
-#[cfg(not(feature = "hacspec"))]
-pub(crate) fn get_receive_invoker_hacspec(start: PublicByteSeq) -> PublicByteSeq {
-    let temp = &mut coerce_hacspec_to_rust_public_byte_seq(start.clone())[..];
-    get_receive_invoker_creusot(temp.as_mut_ptr());
-    coerce_rust_to_hacspec_public_byte_seq(&temp)
-}
-
-#[cfg(not(feature = "hacspec"))]
 extern "C" {
   /// Address of the contract itself, ContractAddress.
   pub(crate) fn get_receive_self_address(start: *mut u8);
 }
 
-#[cfg(not(feature = "hacspec"))]
-#[trusted]
-pub(crate) fn get_receive_self_address_creusot(start: *mut u8) {
-    unsafe { get_receive_self_address(start) }
-}
-
-#[cfg(feature = "hacspec")]
-pub(crate) fn get_receive_self_address_hacspec(start: PublicByteSeq) -> PublicByteSeq {
-    start
-}
-
-#[cfg(not(feature = "hacspec"))]
-pub(crate) fn get_receive_self_address_hacspec(start: PublicByteSeq) -> PublicByteSeq {
-    let temp = &mut coerce_hacspec_to_rust_public_byte_seq(start.clone())[..];
-    get_receive_self_address_creusot(temp.as_mut_ptr());
-    coerce_rust_to_hacspec_public_byte_seq(&temp)
-}
-
-#[cfg(not(feature = "hacspec"))]
 extern "C" {
   /// Self-balance of the contract, returns the amount
   pub(crate) fn get_receive_self_balance() -> u64;
 }
 
-#[cfg(not(feature = "hacspec"))]
-#[trusted]
-pub(crate) fn get_receive_self_balance_creusot() -> u64 {
-    unsafe { get_receive_self_balance() }
-}
-
-#[cfg(feature = "hacspec")]
-pub(crate) fn get_receive_self_balance_hacspec() -> u64 {
-    1u64
-}
-
-#[cfg(not(feature = "hacspec"))]
-pub(crate) fn get_receive_self_balance_hacspec() -> u64 {
-    get_receive_self_balance_creusot()
-}
-
-#[cfg(not(feature = "hacspec"))]
 extern "C" {
   /// Immediate sender of the message (either contract or account).
   pub(crate) fn get_receive_sender(start: *mut u8);
 }
 
-#[cfg(not(feature = "hacspec"))]
-#[trusted]
-pub(crate) fn get_receive_sender_creusot(start: *mut u8) {
-    unsafe { get_receive_sender(start) }
-}
-
-#[cfg(feature = "hacspec")]
-pub(crate) fn get_receive_sender_hacspec(start: PublicByteSeq) -> PublicByteSeq {
-    start
-}
-
-#[cfg(not(feature = "hacspec"))]
-pub(crate) fn get_receive_sender_hacspec(start: PublicByteSeq) -> PublicByteSeq {
-    let temp = &mut coerce_hacspec_to_rust_public_byte_seq(start.clone())[..];
-    get_receive_sender_creusot(temp.as_mut_ptr());
-    coerce_rust_to_hacspec_public_byte_seq(&temp)
-}
-
-#[cfg(not(feature = "hacspec"))]
 extern "C" {
   // Getters for the chain meta data
   /// Slot time (in milliseconds) from chain meta data
   pub(crate) fn get_slot_time() -> u64;
-}
-
-#[cfg(not(feature = "hacspec"))]
-#[trusted]
-pub(crate) fn get_slot_time_creusot() -> u64 {
-    unsafe { get_slot_time() }
-}
-
-#[cfg(feature = "hacspec")]
-pub(crate) fn get_slot_time_hacspec() -> u64 {
-    1u64
-}
-
-#[cfg(not(feature = "hacspec"))]
-pub(crate) fn get_slot_time_hacspec() -> u64 {
-    get_slot_time_creusot()
 }
